add handshake example

theories/Defun.v
@@ -78,12 +78,6 @@ Inductive equiv (state a : Type)(step : state -> step_range state) :
     forall (current : state)(x : a),
       step current = None ->
       equiv step current (Pure _ x)
-| EquivStateSkip :
-    forall (current : state)(T : Type)(f : T -> state)(e : t effect a),
-      step current
-      = Some (existT _ _(skipE T tt, f)) ->
-      (forall x:T, equiv step (f x) e) ->
-      equiv step current e
 | EquivGeneralize :
     forall (current : state)(T : Type)(x0 : T)(f : T -> state)(e' : T -> t effect a) e,
       step current
@@ -92,6 +86,17 @@ Inductive equiv (state a : Type)(step : state -> step_range state) :
       (forall x:T, equiv step (f x) (e' x)) ->
       equiv step current e.
 
+
+Lemma EquivStateSkip :
+  forall state a (step : state -> step_range state) (current : state)(next : state)(e : t effect a),
+    step current
+    = Some (existT _ _ (skipE unit tt, (fun _:unit => next))) ->
+    equiv step next e ->
+    equiv step current e.
+Proof.
+  intros.
+  eapply (EquivGeneralize _ tt (fun _:unit => e)); eauto.
+Qed.
 
 Ltac context_of_aux t1 t2 ctx result :=
   match t1 with
@@ -163,7 +168,7 @@ Ltac unify_fun :=
   simpl;
   repeat curry_lhs;
   let rec unify_fun_aux :=
-      match goal with
+      lazymatch goal with
         |- _ ?x = _ =>
         pattern_rhs x;
         apply equal_f;
@@ -202,7 +207,7 @@ Ltac skip_to env nextptr :=
     let step_f := ptr_to_step_f ptr in
     let ty_env := type of env in
     let f := open_constr:(_  : ty_env -> step_range state) in
-    eapply (@EquivStateSkip _ _ (step_f f) (ptr env) _ nextptr)
+    eapply (@EquivStateSkip _ _ (step_f f) (ptr env) nextptr)
   end.
 
 Ltac is_concr_nat n :=
@@ -211,139 +216,10 @@ Ltac is_concr_nat n :=
   | O => idtac
   end.
 
-Ltac derive env :=
-  lazymatch goal with
-    |- @equiv ?state ?a ?step ?current ?prog =>
-    let ptr := open_constr:(?[ptr]) in
-    context_of current open_constr:(inl _) ptr;
-    let ty_env := type of env in
-    lazymatch prog with
-    | Eff (getE tt) _ =>
-      let env_f' :=
-          lazymatch env with
-          | tt => open_constr:(fun n:nat => n)
-          | _ => open_constr:(fun n:nat => (env,n))
-          end
-      in
-      let step_f := ptr_to_step_f ptr in
-      let f := open_constr:(_  : ty_env -> step_range state) in
-      let f' := open_constr:(_) in
-      eapply (@EquivEffGet _ _ (step_f (f ||| f')) (ptr (inl env))
-                           (fun n => ptr (inr (inl (env_f' n)))));
-      [unify_fun|
-       let n := fresh "n" in
-       intro n; derive constr:(env_f' n)]
-    | Eff (putE ?n) ?e =>
-      let step_f := ptr_to_step_f ptr in
-      let f  := open_constr:(_ : ty_env -> step_range state) in
-      lazymatch e with
-      | (fun _ => Pure _ _) =>
-        eapply (@EquivEffPut _ _ (step_f (f ||| (fun _ => None))) (ptr (inl env))
-                             (fun _ => ptr (inr env)));
-        [try unify_fun|eapply EquivPure; auto]
-      | _ =>
-        let f' := open_constr:(_) in
-        eapply (@EquivEffPut _ _ (step_f (f ||| f')) (ptr (inl env))
-                             (fun _ => ptr (inr (inl env))));
-        [unify_fun|derive env]
-      end
-    | (match ?m with | O => ?progO | S _ => ?progS end) =>
-      let step_f := ptr_to_step_f ptr in
-      let f := open_constr:(_  : ty_env -> step_range state) in
-      let f' := open_constr:(_) in
-      let env' := (eval simpl in env) in
-      let env0 := env_subst env' m 0 in
-      eapply (@EquivStateSkip _ _ (step_f (f ||| f')) (ptr (inl env)) unit
-                              (fun _ => match m with
-                                        | O =>
-                                          ptr (inr (inl (inl env0)))
-                                        | S m' =>
-                                          ptr (inr (inr (@inl nat _ _)))
-                                        end));
-      [ unify_fun
-      | let m' := fresh "m'" in
-        destruct m as [|m'];
-        [ derive env0 | let envm' := env_subst env' m m' in derive envm' ]
-      ]
-    | _ =>
-      let p := leftmost prog in
-      tryif is_fix p then
-        (skip_to env open_constr:(fun _:unit => ptr (inr env));
-         intros;
-         [unify_fun
-         | skip_to env open_constr:(fun _:unit => _);
-           intros;
-           [unify_fun|progress repeat match goal with H : _ |- _ => refine (H _) end]])
-        || (
-          let step_f := ptr_to_step_f ptr in
-          let f := open_constr:(_  : ty_env -> step_range state) in
-          let f' := open_constr:(_) in
-          let env' := (eval simpl in env) in
-          let m := match prog with _ ?k => k end in
-          let env0 := match type of m with
-                      | nat => env_subst env' m 0
-                      | list ?A => env_subst env' m (@nil A)
-                      end
-          in
-          let k := fresh "k" in
-          let rec generalize_args e tac :=
-              lazymatch e with
-              | ?e' m =>
-                lazymatch p with
-                | context[m] =>
-                  eapply (@EquivGeneralize _ _ (step_f (f ||| f')) (ptr (inl env)) _ m (fun k:nat => match m with
-                                                                                                   | O => ptr (inr (inl (inl (env0,k))))
-                                                                                                   | S m' => ptr (inr (inr (inl (_, k))))
-                                                                                                   end));
-                  [ unify_fun
-                  | match goal with
-                      |- ?e ?x = ?f ?x =>
-                      match eval pattern x in f with
-                        ?g _ => exact (eq_refl: e x = (fun y => g y x) x)
-                      end
-                    end
-                  | let m' := fresh "n'" in
-                  induction m as [|m'];
-                  intro k;
-                  simpl;
-                  [ tac env0 0
-                  | tac env' m' ]
-                  ]
-                | _ =>
-                  generalize_args e' tac
-                end
-              | ?e' ?x =>
-                eapply (@EquivGeneralize _ _ (step_f (f ||| f')) (ptr (inl env)) _ x (fun k:nat => match m with
-                                                                                                   | O => ptr (inr (inl (inl (env0,k))))
-                                                                                                   | S m' => ptr (inr (inr (inl (_, k))))
-                                                                                                   end));
-                [ unify_fun
-                | generalize x;
-                  intros;
-                  lazymatch goal with
-                    |- _ ?x = _ =>
-                    pattern_rhs x;
-                    try apply eq_refl
-                  | _ => idtac
-                  end
-                | let m' := fresh "n'" in
-                  induction m as [|m'];
-                  intro k;
-                  simpl;
-                  [ tac env0 0
-                  | tac env' m' ]
-                ]
-              | _ => idtac
-              end
-          in
-          generalize_args prog ltac:(fun env m' =>
-                                       let envm' := env_subst env' m m' in
-                                       derive (envm',k))
-        )
-     else fail 0
-    end
-  end.
+Definition label (A : Type)(x : A) := True.
 
+Ltac set_label env :=
+  assert (label env) by (unfold label; auto).
 
 Ltac derive_step env :=
   lazymatch goal with
@@ -364,12 +240,14 @@ Ltac derive_step env :=
       let f' := open_constr:(_) in
       eapply (@EquivEffGet _ _ (step_f (f ||| f')) (ptr (inl env))
                            (fun n => ptr (inr (inl (env_f' n)))));
-      [unify_fun|
-       let n := fresh "n" in
-       intro n]
+      [unify_fun
+      |let n := fresh "n" in
+       intro n;
+       set_label (env_f' n)
+      ]
     | Eff (putE ?n) ?e =>
       let step_f := ptr_to_step_f ptr in
-      let f  := open_constr:(_ : ty_env -> step_range state a) in
+      let f  := open_constr:(_ : ty_env -> step_range state) in
       lazymatch e with
       | (fun _ => Pure _ _) =>
         eapply (@EquivEffPut _ _ (step_f (f ||| (fun _ => None))) (ptr (inl env))
@@ -379,7 +257,9 @@ Ltac derive_step env :=
         let f' := open_constr:(_) in
         eapply (@EquivEffPut _ _ (step_f (f ||| f')) (ptr (inl env))
                              (fun _ => ptr (inr (inl env))));
-        [unify_fun|]
+        [ unify_fun
+        | assert (label env) by (unfold label; auto)
+        ]
       end
     | (match ?m with | O => ?progO | S _ => ?progS end) =>
       let step_f := ptr_to_step_f ptr in
@@ -387,47 +267,59 @@ Ltac derive_step env :=
       let f' := open_constr:(_) in
       let env' := (eval simpl in env) in
       let env0 := env_subst env' m 0 in
-      eapply (@EquivStateSkip _ _ (step_f (f ||| f')) (ptr (inl env)) unit
-                              (fun _ => match m with
-                                        | O =>
-                                          ptr (inr (inl (inl env0)))
-                                        | S m' =>
-                                          ptr (inr (inr (@inl nat _ _)))
-                                        end));
+      eapply (@EquivStateSkip _ _ (step_f (f ||| f')) (ptr (inl env))
+                              (match m with
+                               | O =>
+                                 ptr (inr (inl (inl env0)))
+                               | S m' =>
+                                 ptr (inr (inr (@inl nat _ _)))
+                               end));
       [ unify_fun
       | let m' := fresh "m'" in
-        destruct m as [|m']
+        destruct m as [|m'];
+        [ assert (label env0) by (unfold label; auto)
+        | let envm' := env_subst env' m m' in
+          assert (label envm')
+        ]
       ]
     | _ =>
       let p := leftmost prog in
       tryif is_fix p then
-        (skip_to env open_constr:(fun _:unit => ptr (inr env));
+        (skip_to env open_constr:(ptr (inr env));
          intros;
          [ unify_fun
-         | skip_to env open_constr:(fun _:unit => _);
+         | skip_to env open_constr:(_);
           intros;
-          [unify_fun|progress eauto]])
+           [unify_fun|progress repeat match goal with H : _ |- _ => refine (H _) || eapply H end]])
         || (
           let step_f := ptr_to_step_f ptr in
-            let f := open_constr:(_  : ty_env -> step_range state) in
-            let f' := open_constr:(_) in
-            let env' := (eval simpl in env) in
-            let m := match prog with _ ?k => k end in
-            let env0 := match type of m with
-                        | nat => env_subst env' m 0
-                        | list ?A => env_subst env' m (@nil A)
-                        end
-            in
-            
+          let f := open_constr:(_  : ty_env -> step_range state) in
+          let f' := open_constr:(_) in
+          let env' := (eval simpl in env) in
+          let m := match prog with _ ?k => k end in
+          let env0 := match type of m with
+                      | nat => env_subst env' m 0
+                      | list ?A => env_subst env' m (@nil A)
+                      end
+          in
+          let k := fresh in
           let rec generalize_args e tac :=
               lazymatch e with
               | ?e' m =>
                 lazymatch p with
                 | context[m] =>
-                  eapply (@EquivGeneralize _ _ (step_f (f ||| f')) (ptr (inl env)) _ m (fun k:nat => match m with
-                                                                                                   | O => ptr (inr (inl (inl (env0,k))))
-                                                                                                   | S m' => ptr (inr (inr (inl (_, k))))
-                                                                                                   end));
+                  match type of m with
+                  | nat =>
+                    eapply (@EquivGeneralize _ _ (step_f (f ||| f')) (ptr (inl env)) _ m (fun k:nat => match m with
+                                                                                                       | O => ptr (inr (inl (inl (env0,k))))
+                                                                                                       | S m' => ptr (inr (inr (inl (_, k))))
+                                                                                                       end))
+                  | list ?A =>
+                    eapply (@EquivGeneralize _ _ (step_f (f ||| f')) (ptr (inl env)) _ m (fun l:list nat => match m with
+                                                                                                            | [] => ptr (inr (inl (inl (env0,l))))
+                                                                                                            | a::l' => ptr (inr (inr (inl (_,l))))
+                                                                                                            end))
+                  end;
                   [ unify_fun
                   | match goal with
                       |- ?e ?x = ?f ?x =>
@@ -435,7 +327,12 @@ Ltac derive_step env :=
                         ?g _ => exact (eq_refl: e x = (fun y => g y x) x)
                       end
                     end
-                  |
+                  | let m' := fresh m "n'" in
+                    induction m as [|m'];
+                    intro k;
+                    simpl;
+                    [ tac env0 0
+                    | tac env' m']
                   ]
                 | _ =>
                   generalize_args e' tac
@@ -446,22 +343,71 @@ Ltac derive_step env :=
                                                                                                    | S m' => ptr (inr (inr (inl (_, k))))
                                                                                                    end));
                 [ unify_fun
-                | generalize x; try reflexivity
-                | let m' := fresh "n'" in
+                | generalize x;
+                  intros;
+                  lazymatch goal with
+                    |- _ ?x = _ =>
+                    pattern_rhs x;
+                    try apply eq_refl
+                  | _ => idtac
+                  end
+                | let m' := fresh m "m'" in
                   induction m as [|m'];
+                  intro k;
+                  simpl;
                   [ tac env0 0
                   | tac env' m' ]
                 ]
-              | _ => idtac
+              | _ =>
+                match type of m with
+                | nat =>
+                  eapply (@EquivStateSkip _ _ (step_f (f ||| f')) (ptr (inl env)) (match m with
+                                                                                                     | O => ptr (inr (inl (inl (env0))))
+                                                                                                     | S m' => ptr (inr (inr (inl _)))
+                                                                                                     end))
+                | list ?A =>
+                  eapply (@EquivStateSkip _ _ (step_f (f ||| f')) (ptr (inl env)) (match m with
+                                                                                                          | [] => ptr (inr (inl (inl env0)))
+                                                                                                          | x::l' => ptr (inr (inr (inl _)))
+                                                                                                          end))
+                end;
+                [ unify_fun
+                | let m' := fresh "n'" in
+                  match type of m with
+                  | nat =>
+                    induction m as [|m'];
+                    [ assert (label env0) by (unfold label; auto)
+                    | let envm' := env_subst env' m m' in
+                      assert (label envm') by (unfold label; auto) ]
+                  | list nat =>
+                    let a := fresh "a" in
+                    induction m as [|a m'];
+                    [ assert (label env0) by (unfold label; auto)
+                    | let envm' := env_subst env' m m' in
+                      assert (label (envm',a)) by (unfold label; auto) ]
+                  end
+                ]
               end
           in
           generalize_args prog ltac:(fun env m' =>
-                                       let envm' := env_subst env' m m' in
-                                       idtac)
+                                         let envm' := env_subst env' m m' in
+                                         assert (label (envm',k)) by (unfold label; auto))
         )
      else idtac
     end
   end.
+
+Ltac derive' env :=
+  derive_step env;
+  repeat
+     match goal with
+       H : label ?e |- _ => clear H; derive_step e
+     end.
+
+Ltac derive env :=
+  repeat eexists;
+  unshelve derive' env;
+  try exact (fun _ => None); try exact unit.
 
 Definition ex : t effect unit :=
   n <- get;
@@ -474,7 +420,6 @@ Definition ex_derive :
   {state & {step & {init | @equiv state _ step init ex}}}.
 Proof.
   unfold ex.
-  repeat eexists.
   derive tt.
 Defined.
 
@@ -506,7 +451,6 @@ Definition ex3''_derive :
   {state & {step & {init | @equiv state _ step init ex3''}}}.
 Proof.
   unfold ex3'',ex3'.
-  repeat eexists.
   derive tt.
 Defined.
 
@@ -518,9 +462,8 @@ Definition ex3_derive :
   {state & {step & {init | @equiv state _ step init ex3 }}}.
 Proof.
   unfold ex3, ex3'.
-  repeat eexists.
   derive tt.
-Defined.  
+Defined.
 
 Definition ex5 : t effect unit :=
   n <- get;
@@ -534,7 +477,6 @@ Definition ex5_derive :
   { state & { step & { init | @equiv state _ step init ex5 }}}.
 Proof.
   unfold ex5.
-  repeat eexists.
   derive tt.
 Defined.
 
@@ -544,7 +486,7 @@ Definition double_loop : t effect unit :=
   n <- get;
     (fix f m :=
        match m with
-       | O => put 0; Pure _ tt
+       | O => put n; Pure _ tt
        | S m' =>
          x <- get;
            (fix g k :=
@@ -558,24 +500,266 @@ Definition double_loop_derive :
   {state & {step & {init | @equiv state _ step init double_loop}}}.
 Proof.
   unfold double_loop.
-  repeat eexists.
   derive tt.
-  derive_step n.
-  
 Defined.
 
-Definition ex_list : t effect unit :=
+Eval cbv [double_loop double_loop_derive sum_merge prod_curry projT1 projT2] in (projT1 (projT2 double_loop_derive)).
+
+Fixpoint ex_list (l : list nat) : t effect unit :=
+  match l with
+  | [] => put 0; Pure _ tt
+  | x::rest =>
+    put x;
+      ex_list rest
+  end.
+
+Definition ex_list_derive :
+  {state & {step & forall l, {init | @equiv state _ step init (ex_list l)}}}.
+Proof.
+  unfold ex_list.
+  repeat eexists.
+  derive l.
+Defined.
+
+(*
+Section ReadL.
+  Variable f : list nat -> t effect unit.
+  
+  Fixpoint readL n accum :=
+    match n with
+    | O => f accum
+    | S n' =>
+      x <- get;
+        readL n' (accum ++ [x])
+    end.
+*)
+Fixpoint readL (f : list nat -> t effect unit) accum n :=
+  match n with
+  | O => f accum
+  | S n' =>
+    x <- get;
+      readL f (accum ++ [x]) n'
+  end.
+
+Fixpoint printL (e : t effect unit) l :=
+  match l with
+  | [] => e
+  | x::l' =>
+    put x;
+      printL e l'
+  end.
+
+Notation "l <- 'read' n ; e" := (readL (fun l => e) [] n) (at level 100, right associativity).
+Notation "'print' l ; e" := (printL e l) (at level 100, right associativity).
+
+
+Lemma read_derive : forall state step ptr next l0 n init e,
+    init = match n with
+           | O => next l0
+           | S n' => ptr l0 (S n')
+           end->
+    (forall l n, step (ptr l n)
+               = match n with
+                 | O =>  Some (existT _ _ (skipE unit tt, (fun _ => next l)))
+                 | S n' => Some (existT _ _ (getE tt, fun x =>
+                                                match n' with
+                                                | O => next (l++[x])
+                                                | S n'' => ptr (l++[x]) (S n'')
+                                                end))
+                 end) ->
+    (forall l, @equiv state _ step (next l) (e l)) ->
+    @equiv state _ step init (readL e l0 n).
+Proof.
+  intros.
+  subst.
+  unfold readL.
+  revert l0.
+  induction n; intros.
+  auto.
+  eapply EquivEffGet; auto.
+  rewrite (H0 l0 (S n)).
+  simpl.
+  reflexivity.
+  intros.
+  apply IHn.
+Qed.
+
+Lemma print_derive : forall state step ptr next l init e,
+    init = match l with
+           | [] => next
+           | _::_ => ptr l
+           end ->
+    (forall l, step (ptr l)
+               = match l with
+                 | [] =>  Some (existT _ _ (skipE unit tt, (fun _ => next)))
+                 | n::l' => Some (existT _ _ (putE n, fun x =>
+                                                match l' with
+                                                | [] => next
+                                                | _::_ => ptr l'
+                                                end))
+                 end) ->
+    @equiv state _ step next e ->
+    @equiv state _ step init (printL e l).
+Proof.
+  intros.
+  subst.
+  unfold printL.
+  induction l.
+  auto.
+  eapply EquivEffPut.
+  rewrite H0.
+  simpl. reflexivity.
+  apply IHl.
+Qed.
+
+Ltac read_derive env_f :=
+  lazymatch goal with
+    |- @equiv ?state ?a ?step ?current (readL _ _ ?n) =>
+    lazymatch type of (env_f n) with
+      ?ty_env =>
+      let ptr := open_constr:(?[ptr]) in
+      context_of current open_constr:(inl _) ptr;
+      let step_f := ptr_to_step_f ptr in
+      let f := open_constr:(_  : ty_env * list nat -> step_range state) in
+      let f' := open_constr:(_) in
+      let env' := eval simpl in (env_f n) in
+      skip_to env' open_constr:(_);
+      [ unify_fun
+      | eapply (@read_derive _ (step_f (_ ||| (f ||| f'))) (fun l n => ptr (inr (inl (env_f n, l))))
+                             (fun l => ptr (inr (inr (inl (env_f 0,l))))));
+        [ reflexivity
+        | intros; simpl; unify_fun
+        | intros
+        ]
+      ]
+    end
+  end.
+
+Ltac print_derive env_f :=
+  lazymatch goal with
+    |- @equiv ?state ?a ?step ?current (printL _ ?l) =>
+    lazymatch type of (env_f l) with
+      ?ty_env =>
+      let ptr := open_constr:(?[ptr]) in
+      context_of current open_constr:(inl _) ptr;
+      let step_f := ptr_to_step_f ptr in
+      let f := open_constr:(_  : ty_env -> step_range state) in
+      let f' := open_constr:(_) in
+      let env' := eval simpl in (env_f l) in
+      skip_to env' open_constr:(_);
+      [ unify_fun
+      | eapply (@print_derive _ (step_f (_ ||| (f ||| f'))) (fun l => ptr (inr (inl (env_f l))))
+                             (ptr (inr (inr (inl (env_f []))))));
+        [ reflexivity
+        | intros; simpl; try unify_fun
+        | intros
+        ]
+      ]
+    end
+  end.
+
+Definition ex_read_print :=
   n <- get;
-    (fix f l m :=
-       match m with
-       | O => put 0; Pure _ tt
-       | S m' =>
-         x <- get;
-           (fix g l' :=
-              match l' with
-              | [] => f (x::l) m'
-              | a::rest =>
-                put a;
-                  g rest
-              end) l
-       end) [] n.
+    l <- read n;
+    print l;
+    put 0;
+    Pure _ tt.
+
+Definition ex_read_print_derive :
+  {state & {step & {init | @equiv state _ step init ex_read_print}}}.
+Proof.
+  unfold ex_read_print.
+  repeat eexists.
+  derive_step tt.
+  read_derive (fun n:nat => n).
+  print_derive (fun l:list nat => (0,l)).
+  derive (0,@nil nat).
+Defined.
+
+Parameter generateKey : unit -> list nat * list nat.
+Parameter open : list nat -> list nat -> list nat -> list nat.
+Parameter seal : list nat -> list nat -> list nat -> list nat.
+
+
+Fixpoint splitAt A n (l : list A) :=
+  match n with
+  | O => ([], l)
+  | S n' =>
+    match l with
+    | [] => ([], [])
+    | x::l' =>
+      let (l1,l2) := splitAt n' l' in
+      (x::l1, l2)
+    end
+  end.
+
+Definition handshake pk sk :=
+  n <- get;
+  m <- get;
+  let (ourEphemeralPublic,ourEphemeralSecret) := generateKey tt in
+  print ourEphemeralPublic;
+    theirEphemeralPublic <- read n;
+    theirHandshakeSealed <- read m;
+    let theirHandshake :=
+        open theirHandshakeSealed theirEphemeralPublic ourEphemeralSecret
+    in
+    let (theirPK,theirHandshakeRest) := splitAt n theirHandshake in
+    let hs := open theirHandshakeRest theirPK ourEphemeralSecret in
+    let ourHandshake :=
+        pk ++ seal (ourEphemeralPublic ++ theirEphemeralPublic) theirEphemeralPublic sk
+    in
+    print (seal ourHandshake theirPK ourEphemeralSecret);
+      Pure _ tt.
+
+Definition handshake_derive :
+  {state & {step & forall pk sk, {init | @equiv state _ step init  (handshake pk sk)}}}.
+Proof.
+  repeat eexists.
+  unfold handshake.
+  destruct  (generateKey tt).
+  derive_step (pk,sk).
+  clear H.
+  derive_step (pk,sk,n).
+  clear H.
+  eapply (@EquivGeneralize _ _ _ (inr (inr (inl (pk,sk,n,n0)))) _ l (fun l => inr (inr (inr (inl (pk,sk,n,n0,l)))))).
+  simpl.
+  match goal with
+    |- ?step _ = _ =>
+    let e := open_constr:(_|||_) in
+    unify step e
+  end.
+  simpl.
+  unify_fun.
+  pattern_rhs l.
+  apply eq_refl.
+  intros.
+  simpl.
+  print_derive (fun l :list nat => (pk,sk,n,n0,l)).
+  read_derive (fun n:nat => (pk,sk,n,n0,@nil nat)).
+  read_derive (fun n:nat => (pk,sk,0,n,@nil nat,l1)).
+  destruct (splitAt n (open l2 l1 l0)).
+  remember (seal (pk ++ seal (x ++ l1) l1 sk) l3 l0) as l5.
+  eapply (@EquivGeneralize _ _ _ _ _ l5 (fun l5 => inr (inr (inr (inr (inr (inr (inr (inr (inr (inr (inl (pk,sk,0,0,[],l1,l2,l5))))))))))))).
+  simpl.
+  match goal with
+    |- ?step _ = _ =>
+    let e := open_constr:(_|||_) in
+    unify step e
+  end.
+  simpl.
+  unify_fun.
+  pattern_rhs l5.
+  apply eq_refl.
+  simpl.
+  intros.
+  print_derive (fun l:list nat => (pk,sk,0,0,@nil nat,l1,l2,l)).
+  eapply EquivPure.
+  simpl.
+  let e := open_constr:(fun _ => None) in
+  match goal with
+    |- ?g _ = _ => unify g e
+  end.
+  reflexivity.
+  Grab Existential Variables.
+  exact unit.
+Defined.
